For all of the following solutions, by definition of \textit{monotonically increasing}, if $m \leq n$, then:
\begin{eqnarray*}
	f(m) \leq f(n) \\
	g(m) \leq g(n)
\end{eqnarray*}

\begin{itemize}
\item[\textbf{a)}] Let $m \leq n$, then since $f(n)$ and $g(n)$ are monotonically increasing:
	\begin{eqnarray*}
		f(m) + g(m) & \leq & f(n) + g(m) \\
		g(m) + f(m) & \leq & g(n) + f(m) \\
		f(m) + g(n) & \leq & f(n) + g(n) \\
		g(m) + f(n) & \leq & f(n) + g(n)
	\end{eqnarray*}
	Comparing these equations then shows that $f(m) + g(m) \leq f(n) + g(n)$, thus $f(n) + g(n)$ is also monotonically increasing.
\item[\textbf{b)}] Let $m \leq n$, then $g(m) \leq g(n)$ since $g(n)$ is monotonically increasing, and since $f(n)$ is also monotonically increasing, $f(g(m)) \leq f(g(n))$, thus $f(g(n))$ is monotonically increasing.
\item[\textbf{c)}] Let $m \leq n$, then:
	\begin{eqnarray*}
		f(m) \cdot g(m) & \leq & f(n) \cdot g(m) \\
		g(m) \cdot f(m) & \leq & g(n) \cdot f(m) \\
		f(m) \cdot g(n) & \leq & f(n) \cdot g(n) \\
		g(m) \cdot f(n) & \leq & g(n) \cdot f(n)
	\end{eqnarray*}
	Comparing these equations then shows that $f(m) \cdot g(m) \leq g(n) \cdot f(n)$, thus $f(n) \cdot g(n)$ is also monotonically increasing for nonnegative $f(n)$ and $g(n)$.
\end{itemize}
