Using the substitution $T(n) \leq cn^2$, try to prove the Inductive Case for the recurrence $T(n) = 4T(n/2) + n$ by making the assumption that this bound holds for all $m < n$, in particular for $m = n/2$, giving:
\begin{equation*}
	T\left(\frac{n}{2}\right) \leq c\left(\frac{n}{2}\right)^2
\end{equation*}
Substituting into the recurrence then gives:
\begin{eqnarray*}
	T(n) &\leq& 4c\left(\frac{n}{2}\right)^2 + n \\
	 &=& 4c\frac{n^2}{4} + n \\
	 &=& cn^2 + n
\end{eqnarray*}
\ldots which does not hold.  However, using the substitution $T(n) \leq cn^2 - n$ gives the assumption:
\begin{equation*}
	T\left(\frac{n}{2}\right) \leq c\left(\frac{n}{2}\right)^2 - \frac{n}{2}
\end{equation*}
Once more, substituting into the recurrence then gives:
\begin{eqnarray*}
	T(n) &\leq& 4c\left(\frac{n}{2}\right)^2 - 4\left(\frac{n}{2}\right) + n \\
	 &=& 4c \frac{n^2}{4} - 2n + n \\
	 &=& cn^2 - n
\end{eqnarray*}
Thus the Inductive Case holds.

For the Base Case, assume that $T(1) = 1$, then prove:
\begin{eqnarray*}
	T(n) &\leq& cn^2 - n \\
	T(1) = 1 &\leq& c1^2 - 1 \\
	 &\leq& c - 1
\end{eqnarray*}
\ldots which is true for any $c \geq 2$, thus the Base Case holds.

Therefore the substitution proof fails for $T(n) \leq cn^2$ but holds for $T(n) \leq cn^2 - n$.
