Using the substitution $T(n) \leq cn^{\log_3(4)}$, try to prove the Inductive Case for the recurrence $T(n) = 4T(\frac{n}{3}) + n$ by making the assumption that this bound holds for all $m < n$, in particular for $m = n/3$, giving:
\begin{equation*}
	T\left(\frac{n}{3}\right) \leq c\left(\frac{n}{3}\right)^{\log_3(4)}
\end{equation*}
Substituting this into the recurrence then gives:
\begin{eqnarray*}
	T(n) &\leq& 4c\left(\frac{n}{3}\right)^{\log_3(4)} + n \\
	 &=& 4c \cdot \frac{n^{\log_3(4)}}{3^{\log_3(4)}} + n \\
	 &=& 4c \cdot \frac{n^{\log_3(4)}}{4} + n \\
	 &=& cn^{\log_3(4)} + n
\end{eqnarray*}
\ldots this solution does not hold. However, using the substitution $T(n) \leq cn^{\log_3(4)} - 3n$, gives the assumption:
\begin{equation*}
	T\left(\frac{n}{3}\right) \leq c\left(\frac{4}{3}\right)^{\log_3(4)} - n
\end{equation*}
Once more, substituting into the recurrence then gives:
\begin{eqnarray*}
	T(n) &\leq& 4c\left(\frac{n}{3}\right)^{\log_3(4)} - 4n + n \\
	 &=& 4c \cdot \frac{n^{\log_3(4)}}{3^{\log_3(4)}} - 3n \\
	 &=& 4c \cdot \frac{n^{\log_3(4)}}{4} - 3n \\
	 &=& cn^{\log_3(4)} - 3n
\end{eqnarray*}
Thus the Inductive Case holds.

For the Base Case, assume that $T(1) = 1$, then prove:
\begin{eqnarray*}
	T(n) &\leq& cn^{\log_3(4)} - 3n \\
	T(1) = 1 &\leq& c1^{\log_3(4)} - 3\cdot1 \\
	 &\leq& c - 3
\end{eqnarray*}
\ldots which is true for any $c \geq 4$, thus the Base Case holds.

Therefore the substitution proof fails for $T(n) \leq cn^{\log_3(4)}$ but holds for $T(n) \leq cn^{\log_3(4)} - n$.
