Assume a base case of $T(1) = 1$.  The recurrence tree is then:
\begin{center}
\begin{forest}
[$1$,name=level1
	[$1$
		[$1$,for descendants={edge=dotted}
			[]
			[]
			[]
			[]
		][$1$,for descendants={edge=dotted}
			[]
			[]
			[]
			[]
		]
	][$1$,name=level2
		[$1$,for descendants={edge=dotted}
			[]
			[]
			[]
			[]
		][$1$,for descendants={edge=dotted}, name=level3
			[]
			[]
			[]
			[]
		]
	]
]
% Bottom leaves.
\node(bottombox) at ($(current bounding box.south) - (0, 1)$){};
\foreach \x in {-4, -3, ..., 1, 2, 4} {
	\node(leaf\x) at ($(bottombox.west) + (\x, 0)$){$1$};
	\draw[dotted] (leaf\x) -- +(0, 1);
}
\node at ($(bottombox.west) + (3, 0)$){\ldots};
% Left side arrow thingy.
\node(leftbox) at ($(current bounding box.west) - (1.25, 0)$){$n$};
\path (current bounding box.north west) -- (current bounding box.north) node(topline){};
\draw[->] (leftbox) -- (leftbox |- topline);
\path (current bounding box.south west) -- (current bounding box.south) node(botline){};
\draw[->] (leftbox) -- (leftbox |- botline);
% Right side sums.
\path ($(current bounding box.north east) + (0.5, 0)$) -- ($(current bounding box.south east) + (0.5, 0)$) node(rightline){};
\draw[-stealth,dotted,thick] (level1) -- (level1 -| rightline) node(l1node){};
\node at ($(l1node) + (1, 0)$){$1$};
\draw[-stealth,dotted,thick] (level2) -- (level2 -| rightline) node(l2node){};
\node at ($(l2node) + (1, 0)$){$2$};
\draw[-stealth,dotted,thick] (level3) -- (level3 -| rightline) node(l3node){};
\node at ($(l3node) + (1, 0)$){$4$};
\path[] (level4) -- (level4 -| rightline) node(l4node){};
\node at ($(l4node) + (1, 0)$){\vdots};
\draw[-stealth,dotted,thick] (leaf4) -- (leaf4 -| rightline) node(leafnode){};
\node (rightleaftotal) at ($(leafnode) + (1, 0)$){$2^{n-1}$};
\end{forest}
\end{center}
It should be apparent from the recurrence tree that the total cost of a level at height $i$ is $2^i$.  Summing up the total cost of all levels gives:
\begin{eqnarray*}
	\sum_{i=0}^{n-1} 2^i & = & \frac{2^n - 1}{2 - 1} \\
	& = & 2^n - 1
\end{eqnarray*}
This gives a guess of $O(2^n)$.  In order to verify, use the Substitution Method to show that $T(n) \leq n^2 - 1$; assume that this is true for all $m < n$, in particular for $m = n - 1$, then $T(n-1) \leq 2^{n-1} - 1$; substituting this into the recurrence equation gives:
\begin{eqnarray*}
	T(n) & \leq & 2(2^{n-1} - 1) + 1 \\
	& = & 2^n - 2 + 1 \\
	& = & 2^n - 1
\end{eqnarray*}
Thus the inductive case holds.  For the base case:
\begin{eqnarray*}
	T(1) & \leq & 2^1 - 1 \\
	& = & 1
\end{eqnarray*}
Thus the base case holds.  Therefore the recurrence is $O(2^n)$.
