The book states that differentiating the Geometric Series and then multiplying the result by $x$ gives:
\begin{eqnarray*}
	\sum_{k=0}^\infty k x^k & = & \frac{x}{\left ( 1-x \right )^2}
\end{eqnarray*}
\ldots for $\left | x \right | < 1$. Differentiating again gives:
\begin{eqnarray*}
	\partial x \sum_{k=0}^\infty k x^k & = & \partial x \frac{x}{\left ( 1-x \right )^2} \\
	\sum_{k=0}^\infty k^2 x^{k-1} & = & \frac{\left ( 1-x \right )^2 + 2\left ( 1-x \right )x}{\left ( 1-x \right )^4} \\
	& = & \frac{\left ( 1-x \right ) + 2x}{\left ( 1-x \right )^4} \\
	& = & \frac{1+x}{\left ( 1-x \right )^3}
\end{eqnarray*}
Multiplying by $x$ again gives:
\begin{eqnarray*}
	x \sum_{k=0}^\infty k^2 x^{k-1} & = & x \frac{1+x}{\left ( 1-x \right )^3} \\
	\sum_{k=0}^\infty k^2 x^k & = & \frac{x \left ( 1+x \right )}{\left ( 1-x \right )^3}
\end{eqnarray*}
Again, both of these formulas only apply for $\left | x \right | < 1$.
